WIP ftlr EInit attempts 2 steps invariant opening

theories/ftlr/EInit.v
@@ -18,195 +18,957 @@ Section fundamental.
 
   Local Hint Resolve finz_seq_between_NoDup list_remove_elem_NoDup : core.
 
+
   (** Predicate that defines when the contents of a register can be swept;
       i.e. when the register contains a capability with at least R permissions... *)
-  Definition reg_allows_einit
-    (lregs : LReg) (lmem : LMem) (r : RegName)
-    (b e a : Addr) (v : Version)
-    (b' e' a' : Addr) (v' : Version):=
-    lregs !! r = Some (LCap RX b e a v)
-    ∧ lmem !! (a,v) = Some (LCap RW b' e' a' v').
-
-  (* TODO move stdpp_extra *)
-  Fixpoint list_remove_elem_list `{A : Type} `{EqDecision A} (la' la : list A) : list A :=
-    match la' with
-    | [] => la
-    | h::t => list_remove_elem h (list_remove_elem_list t la)
-    end.
+  Definition reg_allows_einit_code
+    (lregs : LReg) (r : RegName)
+    (p : Perm) (b e a : Addr) (v : Version):=
+    lregs !! r = Some (LCap p b e a v) ∧ p = RX.
 
   Definition code_addresses (a_pc : Addr) (code_la : list Addr)
     := (list_remove_elem a_pc code_la).
+  Definition allow_einit_code_mask
+    (a_pc : Addr) (v_pc : Version) (code_la : list Addr) (code_v : Version): coPset :=
+    compute_mask_region (⊤ ∖ ↑logN.@(a_pc, v_pc)) (code_addresses a_pc code_la) code_v.
 
-  Definition allow_einit_mask_code
+  Lemma allow_einit_code_mask_remove_nodup
     (a_pc : Addr) (v_pc : Version)
-    (code_la : list Addr) (code_v : Version)
-    : coPset :=
-    let pc_mask := (⊤ ∖ ↑logN.@(a_pc, v_pc)) in
-    compute_mask_region pc_mask (code_addresses a_pc code_la) code_v.
+    (la_code : list Addr) (v_code : Version) :
+    NoDup la_code ->
+    allow_einit_code_mask a_pc v_pc (code_addresses a_pc la_code) v_code =
+    allow_einit_code_mask a_pc v_pc la_code v_code.
+  Proof.
+    intros HNoDup.
+    by rewrite /allow_einit_code_mask /code_addresses list_remove_elem_idem.
+  Qed.
 
-  Definition data_addresses (a_pc : Addr) (code_la data_la : list Addr)
-    := (list_remove_elem_list (a_pc::code_la) data_la).
 
-  Definition allow_einit_mask_data
-    (a_pc : Addr) (v_pc : Version)
-    (code_la : list Addr) (code_v : Version)
-    (data_la : list Addr) (data_v : Version)
-    : coPset :=
-    let code_mask := allow_einit_mask_code a_pc v_pc code_la code_v in
-    compute_mask_region code_mask (data_addresses a_pc code_la data_la) data_v.
+  Definition interp_list_pred
+    (lws : list LWord) (Ps : list D) (has_later : bool) : iProp Σ :=
+    ([∗ list] lw;Pw ∈ lws;Ps, (if has_later then ▷ (Pw : D) lw else (Pw : D) lw)).
 
-  (* Lemma allow_einit_mask_remove_nodup *)
-  (*   (a_pc : Addr) (v_pc : Version) (code_la data_la : list Addr) (v : Version) : *)
-  (*   NoDup code_la -> *)
-  (*   NoDup data_la -> *)
-  (*   allow_sweep_mask a_pc v_pc (list_remove_elem a_pc la) v = *)
-  (*   allow_sweep_mask a_pc v_pc la v. *)
-  (* Proof. *)
-  (*   intros HNoDup. *)
-  (*   by rewrite /allow_sweep_mask list_remove_elem_idem. *)
-  (* Qed. *)
+  Definition interp_list_persistent
+    (lws : list LWord) (Ps : list D) : iProp Σ :=
+    ( ⌜ Persistent ([∗ list] lw;Pw ∈ lws;Ps, (Pw : D) lw) ⌝ ).
+
+  Definition interp_list_readcond
+    (lws : list LWord) (Ps : list D) (has_later : bool) : iProp Σ :=
+    ( if has_later
+      then [∗ list] Pa ∈ Ps, read_cond Pa interp
+      else [∗ list] Pa ∈ Ps, (□ ∀ (lw : LWord), (Pa : D) lw -∗ interp lw)
+    )%I.
+
+  Definition interp_list_close
+    (la : list Addr) (Ps : list D) (v : Version) (E E' : coPset) : iProp Σ :=
+    ( (▷ ([∗ list] a_Pa ∈ zip la Ps, (interp_ref_inv a_Pa.1 v a_Pa.2))) ={E', E }=∗ True).
 
   (* this will help us close the invariant again... *)
   (* it states which properties are enforced on all the lws *)
-
-
-  Definition region_open_resources
+  Definition resources_open_invariant_code
     (a_pc : Addr) (v_pc : Version)
-    (code_la : list Addr) (code_v : Version)
-    (code_lws : list LWord) (code_Ps : list D)
-    (data_la : list Addr) (data_v : Version)
-    (data_lws : list LWord) (data_Ps : list D)
+    (la_code : list Addr) (v_code : Version)
+    (lws_code : list LWord) (Ps_code : list D)
     (has_later : bool)
     : iProp Σ :=
 
-    let E := ⊤ ∖ ↑logN.@(a_pc, v_pc) in
-    let E1 := allow_einit_mask_code a_pc v_pc code_la code_v in
-    let E2 := allow_einit_mask_data a_pc v_pc code_la code_v data_la data_v in
+    let E0 := ⊤ ∖ ↑logN.@(a_pc, v_pc) in
+    let E1 := allow_einit_code_mask a_pc v_pc la_code v_code in
 
-    ([∗ list] lw;Pw ∈ code_lws;code_Ps, (if has_later then ▷ (Pw : D) lw else (Pw : D) lw))
-    ∗ ([∗ list] lw;Pw ∈ data_lws;data_Ps, (if has_later then ▷▷ (Pw : D) lw else (Pw : D) lw))
+    interp_list_pred lws_code Ps_code has_later
+    ∗ interp_list_persistent lws_code Ps_code
+    ∗ interp_list_readcond lws_code Ps_code has_later
+    ∗ interp_list_close la_code Ps_code v_code E0 E1.
 
-    ∗ ( ⌜ Persistent ([∗ list] lw;Pw ∈ code_lws;code_Ps, (Pw : D) lw) ⌝ ) (* All properties P are persistent *)
-    ∗ ( ⌜ Persistent ([∗ list] lw;Pw ∈ data_lws;data_Ps, (Pw : D) lw) ⌝ ) (* All properties P are persistent *)
+  Definition allows_einit_code (lregs : LReg) (r : RegName) :=
+    ∀ p b e a v,
+    lregs !! r = Some (LCap p b e a v)
+    -> readAllowed p = true
+    -> (finz.seq_between b e) ## reserved_addresses.
 
-    ∗ ( if has_later
-        then ([∗ list] Pa ∈ code_Ps, read_cond Pa interp)
-             ∗ ([∗ list] Pa ∈ data_Ps, ▷ read_cond Pa interp)
-               (* the read cond holds *)
-        else ([∗ list] Pa ∈ code_Ps, (□ ∀ (lw : LWord), (Pa : D) lw -∗ interp lw))
-               ∗ ([∗ list] Pa ∈ data_Ps, (□ ∀ (lw : LWord), (Pa : D) lw -∗ interp lw))
-      )%I
+  Definition allows_einit_data (lmem : LMem) (b : Addr) (v : Version) :=
+    ∀ p' b' e' a' v',
+    lmem !! (b,v) = Some (LCap p' b' e' a' v')
+    -> readAllowed p' = true
+    -> (finz.seq_between b' e') ## reserved_addresses.
 
-    ∗ (▷▷ ([∗ list] a_Pa ∈ zip data_la code_Ps, (interp_ref_inv a_Pa.1 data_v a_Pa.2)) ={E2, E1 }=∗ True)
-    ∗ (▷ ([∗ list] a_Pa ∈ zip code_la data_Ps, (interp_ref_inv a_Pa.1 code_v a_Pa.2)) ={E1, E }=∗ True).
-
-  Definition einit_mask_cond
-    (lregs : LReg) (lmem : LMem)
-    (src : RegName) (b_src e_src a_src : Addr) (v_src : Version)
-    (b' e' a' : Addr) (v' : Version)
+  Definition einit_code_mask_cond
+    (lregs : LReg) (src : RegName)
+    (p_code : Perm) (b_code e_code a_code : Addr) (v_code : Version)
     (a_pc : Addr) (v_pc : Version) :=
-    (* TODO it misses something here: we need conditions over a_pc and b' e' *)
-    decide (reg_allows_einit lregs lmem src b_src e_src a_src v_src b' e' a' v'
-            /\ (src = PC \/ a_pc ∉ (finz.seq_between b_src e_src))
-      ).
+    decide (reg_allows_einit_code lregs src p_code b_code e_code a_code v_code
+            /\ (src = PC \/ a_pc ∉ (finz.seq_between b_code e_code))).
 
-  (* Description of what the resources are supposed to look like after opening the region *)
-  (*    if we need to, but before closing the region up again*)
-
-  Definition allow_einit_res
-    (lregs : LReg) (lmem : LMem)
-    (src : RegName)
+  Definition allow_einit_code_resources
+    (lregs : LReg) (src : RegName)
     (a_pc : Addr) (v_pc : Version)
-    (b_code e_code a_code : Addr) (v_code : Version) (code_Ps : list D)
-    (b_data e_data a_data : Addr) (v_data : Version) (data_Ps : list D)
+    (p_code : Perm) (b_code e_code a_code : Addr) (v_code : Version) (Ps_code : list D)
     :=
 
-    let code_la  := code_addresses a_pc (finz.seq_between b_code e_code) in
-    let data_la  := data_addresses a_pc code_la (finz.seq_between b_data e_data) in
-    let E   := ⊤ ∖ ↑logN.@(a_pc, v_pc) in
-    let E1 := allow_einit_mask_code a_pc v_pc code_la v_code in
-    let E2 := allow_einit_mask_data a_pc v_pc code_la v_code data_la v_data in
+    let la_code  := code_addresses a_pc (finz.seq_between b_code e_code) in
+    let E0 := ⊤ ∖ ↑logN.@(a_pc, v_pc) in
+    let E1 := allow_einit_code_mask a_pc v_pc la_code v_code in
 
-    (⌜read_reg_inr lregs src RX b_code e_code a_code v_code⌝ ∗
-     ⌜allows_einit lregs lmem src⌝ ∗
-     if einit_mask_cond lregs lmem
-          src b_code e_code a_code v_code
-          b_data e_data a_data v_data
-          a_pc v_pc
+    (⌜read_reg_inr lregs src p_code b_code e_code a_code v_code⌝ ∗
+     ⌜allows_einit_code lregs src⌝ ∗
+     if einit_code_mask_cond lregs src p_code b_code e_code a_code v_code a_pc v_pc
      then
-      (|={E, E2}=> (* we open this invariant with all the points-tos from b to e *)
-         ∃ (code_lws : list LWord) (data_lws : list LWord),
-         ⌜ length code_lws = length code_la ⌝
-         ∗ ⌜ length data_lws = length data_la ⌝
-         ∗ ([∗ map] la↦lw ∈ (logical_region_map code_la code_lws v_code), la ↦ₐ lw) (* here you get all the points-tos *)
-         ∗ ([∗ map] la↦lw ∈ (logical_region_map data_la data_lws v_data), la ↦ₐ lw)
-         ∗ region_open_resources a_pc v_pc
-             code_la v_code code_lws code_Ps
-             data_la v_data data_lws data_Ps
-             true)%I
+      (|={E0, E1}=> (* we open this invariant with all the points-tos from b to e *)
+         ∃ (lws_code :list LWord),
+         ⌜ length lws_code = length la_code ⌝
+         ∗ ([∗ map] la↦lw ∈ (logical_region_map la_code lws_code v_code), la ↦ₐ lw) (* here you get all the points-tos *)
+         ∗ resources_open_invariant_code a_pc v_pc la_code v_code lws_code Ps_code true)%I
      else True)%I.
 
-  (* this does not yet open the invariant *)
-  Lemma create_einit_res
-    (lregs : LReg) (lmem : LMem)
-    (src : RegName)
+
+  Lemma create_einit_code_resources
+    (lregs : LReg) (src : RegName)
     (p_pc : Perm) (b_pc e_pc a_pc : Addr) (v_pc : Version)
-    (b_code e_code a_code : Addr) (v_code : Version)
-    (b_data e_data a_data : Addr) (v_data : Version) :
+    (p_code : Perm) (b_code e_code a_code : Addr) (v_code : Version) :
 
-    let code_la  := code_addresses a_pc (finz.seq_between b_code e_code) in
-    let data_la  := data_addresses a_pc code_la (finz.seq_between b_data e_data) in
+    let la_code  := code_addresses a_pc (finz.seq_between b_code e_code) in
 
-    read_reg_inr (<[PC:=LCap p_pc b_pc e_pc a_pc v_pc]> lregs) src RX b_code e_code a_code v_code
+    read_reg_inr (<[PC:=LCap p_pc b_pc e_pc a_pc v_pc]> lregs) src p_code b_code e_code a_code v_code
     -> a_pc ∈ finz.seq_between b_pc e_pc
     → (∀ (r : RegName) lw, ⌜r ≠ PC⌝ → ⌜lregs !! r = Some lw⌝ → (fixpoint interp1) lw)
     -∗ interp (LCap p_pc b_pc e_pc a_pc v_pc)
-    -∗ (∃ (code_Ps : list D) (data_Ps  : list D),
-           ⌜ length code_la = length code_Ps ⌝
-           ∗ ⌜length data_la = length data_Ps ⌝
-           ∗ allow_einit_res
-               (<[PC:=LCap p_pc b_pc e_pc a_pc v_pc]> lregs) lmem src
+    -∗ (∃ (Ps_code : list D),
+           ⌜ length la_code = length Ps_code ⌝
+           ∗ allow_einit_code_resources
+               (<[PC:=LCap p_pc b_pc e_pc a_pc v_pc]> lregs) src
                a_pc v_pc
-               b_code e_code a_code v_code code_Ps
-               b_data e_data a_data v_data data_Ps
-       ).
+               p_code b_code e_code a_code v_code Ps_code).
   Proof.
-  Admitted.
+    intros * Hread Hapc_inbounds.
+    iIntros "#Hreg #Hinterp_pc".
+    apply list_remove_elem_in in Hapc_inbounds.
+    destruct Hapc_inbounds as (la' & <- & Hapc_inbounds).
+    rewrite /allow_einit_code_resources /einit_code_mask_cond.
+    case_decide as Hallows; cycle 1.
+    { iExists (repeat (λne _, True%I) (length la_code)); iFrame "%".
+      iSplit; first by rewrite repeat_length.
+      iSplit; last done.
+      iIntros (p b e a v Hlv HreadAllowed).
+      destruct (decide (src = PC)) as [-> | Hneq_src_pc] ; simplify_map_eq.
+      + iDestruct (readAllowed_not_reserved with "Hinterp_pc") as "%"; auto.
+      + iAssert (interp (LCap p b e a v)) as "Hinterp_src".
+        { iApply "Hreg"; eauto. }
+        iDestruct (readAllowed_not_reserved with "Hinterp_src") as "%"; auto.
+    }
+    iFrame "%".
+    cbn in Hapc_inbounds.
+    apply bind_Some in Hapc_inbounds.
+    destruct Hapc_inbounds as (? & Hrem & ?) ; simplify_eq.
+    rewrite /reg_allows_einit_code in Hallows.
+    destruct Hallows as ( (Hreg & HreadAllowed) & Hdecide).
+    assert (la_code ⊆+ finz.seq_between b_code e_code)
+      as Hla_subseteq by apply list_remove_elem_submsteq.
+    assert (NoDup la_code) as Hla_NoDup by (by apply list_remove_elem_NoDup).
+    rewrite /read_reg_inr in Hread; simplify_map_eq.
 
-  Definition allow_einit_mem
+    destruct (decide (src = PC)) as [-> | Hneq_src_pc] ; simplify_map_eq.
+    (* src = PC *)
+    - rewrite /allow_einit_code_mask /code_addresses.
+      rewrite list_remove_elem_idem; last done.
+      iDestruct (interp_open_region $ (⊤ ∖ ↑logN.@(a_code, v_code)) with "Hinterp_pc")
+        as (Ps) "[%Hlen_Ps Hmod]" ; eauto.
+      { eapply Forall_forall. intros a' Ha'.
+        subst la_code.
+        eapply namespaces.coPset_subseteq_difference_r; auto.
+        assert (a' ≠ a_code).
+        {
+          eapply list_remove_elem_neq; cycle 1 ; eauto.
+          apply list_remove_Some in Hrem.
+          setoid_rewrite Hrem; set_solver.
+        }
+        solve_ndisj.
+      }
+      iExists Ps.
+      iSplit ; first by subst.
+      iSplit.
+      { iIntros (p b e a v Hsrc HreadAllowedp).
+        iDestruct (readAllowed_not_reserved with "Hinterp_pc") as "%"; auto.
+        by simplify_map_eq.
+      }
+      iMod "Hmod".
+      iDestruct "Hmod" as (lws) "(%Hlws & %Hpers & Hmem & HPs & HPs' & Hclose)".
+      iExists lws.
+      iFrame; iFrame "%".
+      iModIntro.
+      iIntros "H".
+      iDestruct ("Hclose" with "H") as "Hclose".
+      rewrite /allow_einit_code_mask /code_addresses.
+      rewrite list_remove_elem_notin.
+      subst la_code.
+      iFrame.
+      apply not_elemof_list_remove_elem; done.
+
+    (* src ≠ PC *)
+    - destruct Hdecide as [Hcontra|Ha_notin_rem] ; first contradiction.
+      iAssert (interp (LCap RX b_code e_code a_code v_code)) as "#Hinterp_code"
+      ; first (iApply "Hreg"; eauto).
+      iDestruct (interp_open_region $ (⊤ ∖ ↑logN.@(a_pc, v_pc)) with "Hinterp_code")
+        as (Ps) "[%Hlen_Ps Hmod]" ; eauto.
+      { apply Forall_forall; intros a' Ha'.
+        subst la_code.
+        assert (a' ≠ a_pc).
+        { intro ; subst. by apply not_elemof_list_remove_elem in Ha'. }
+        apply namespaces.coPset_subseteq_difference_r; [solve_ndisj|set_solver].
+      }
+      iExists Ps.
+      iSplit ; first by subst.
+      iSplit.
+      { iIntros (p b e a v Hsrc HreadAllowedp).
+        iDestruct (readAllowed_not_reserved with "Hinterp_code") as "%"; auto.
+        by simplify_map_eq.
+      }
+      iMod "Hmod".
+      rewrite allow_einit_code_mask_remove_nodup; auto.
+      iDestruct "Hmod" as (lws) "(%Hlws & %Hpers & Hmem & HPs & HPs' & Hclose)".
+      iExists lws.
+      iFrame; iFrame "%".
+      iModIntro.
+      iIntros "H".
+      iDestruct ("Hclose" with "H") as "Hclose".
+      by rewrite allow_einit_code_mask_remove_nodup.
+  Qed.
+
+  Definition allow_einit_code_mem
     (lmem : LMem) (lregs : LReg) (src : RegName)
     (a_pc : Addr) (v_pc : Version) (lw_pc : LWord)
-
-    (b_code e_code a_code : Addr) (v_code : Version) (code_Ps : list D)
-    (b_data e_data a_data : Addr) (v_data : Version) (data_Ps : list D)
-
+    (p_code : Perm) (b_code e_code a_code : Addr) (v_code : Version) (Ps_code : list D)
     (has_later : bool) :=
 
-    let code_la  := code_addresses a_pc (finz.seq_between b_code e_code) in
-    let data_la  := data_addresses a_pc code_la (finz.seq_between b_data e_data) in
+    let la_code  := code_addresses a_pc (finz.seq_between b_code e_code) in
 
-    (⌜read_reg_inr lregs src RX b_code e_code a_code v_code⌝ ∗
-     if einit_mask_cond lregs lmem
-          src b_code e_code a_code v_code
-          b_data e_data a_data v_data
-          a_pc v_pc
-     then (∃ (code_lws : list LWord) (data_lws : list LWord),
-           ⌜ length code_la = length code_lws ⌝
-           ∗ ⌜length data_la = length data_lws ⌝
-           ∗ ⌜lmem = <[(a_pc, v_pc):=lw_pc]>
-                       (logical_region_map code_la code_lws v_code
-                          ∪ logical_region_map data_la data_lws v_data)⌝
-              ∗ region_open_resources a_pc v_pc
-                  code_la v_code code_lws code_Ps
-                  data_la v_data data_lws data_Ps
-                  has_later)
+    (⌜read_reg_inr lregs src p_code b_code e_code a_code v_code⌝ ∗
+     if einit_code_mask_cond lregs src p_code b_code e_code a_code v_code a_pc v_pc
+     then (∃ (lws_code : list LWord),
+              ⌜length lws_code = length la_code⌝
+              ∗ ⌜lmem = <[(a_pc, v_pc):=lw_pc]> (logical_region_map la_code lws_code v_code)⌝
+              ∗ resources_open_invariant_code a_pc v_pc la_code v_code lws_code Ps_code has_later)%I
      else ⌜lmem = <[(a_pc, v_pc):=lw_pc]> ∅⌝)%I.
 
-  Lemma einit_case (lregs : leibnizO LReg)
-    (p : Perm) (b e a : Addr) (v : Version)
-    (lw : LWord) (r : RegName) (P : D):
-    ftlr_instr lregs p b e a v lw (EInit r) P.
+  Lemma einit_code_resources_implies_mem_map
+    (lregs : LReg) (src : RegName)
+    (a_pc : Addr) (v_pc : Version) (lw_pc : LWord)
+    (p_code : Perm) (b_code e_code a_code : Addr) (v_code : Version) (Ps_code : list D)
+    :
+
+    let la_code  := code_addresses a_pc (finz.seq_between b_code e_code) in
+    let E0 := ⊤ ∖ ↑logN.@(a_pc, v_pc) in
+    let E1 := allow_einit_code_mask a_pc v_pc la_code v_code in
+
+    allow_einit_code_resources lregs src a_pc v_pc p_code b_code e_code a_code v_code Ps_code
+    -∗ (a_pc, v_pc) ↦ₐ lw_pc
+    ={ E0,
+         if einit_code_mask_cond lregs src p_code b_code e_code a_code v_code a_pc v_pc
+         then E1
+         else E0
+      }=∗
+    ∃ lmem : LMem,
+      allow_einit_code_mem lmem lregs src a_pc v_pc lw_pc p_code b_code e_code a_code v_code Ps_code true
+      ∗ ([∗ map] la↦lw ∈ lmem, la ↦ₐ lw).
   Proof.
+    intros *.
+    iIntros "HSweepRes Ha_pc".
+    iDestruct "HSweepRes" as "(%Hread & [ %Hreserved HSweepRes ] )".
+    subst E1.
+    rewrite /einit_code_mask_cond.
+    case_decide as Hallows; cycle 1.
+      - iExists _.
+        iSplitR "Ha_pc".
+        + iFrame "%".
+          rewrite /einit_code_mask_cond; case_decide; first by exfalso. auto.
+        + iModIntro. by iApply memMap_resource_1.
+      - iMod "HSweepRes" as (lws) "(%Hlws & Hmem & HSweepRest)".
+        iExists _.
+        iSplitL "HSweepRest".
+        * iFrame "%".
+          rewrite decide_True; auto.
+        * iModIntro.
+          destruct Hallows as ((Hrinr & Hra) & Hne).
+          iDestruct (big_sepM_insert with "[$Hmem $Ha_pc]") as "Hmem" ; cycle 1 ; auto.
+          rewrite /logical_region_map.
+          apply not_elem_of_list_to_map_1.
+          rewrite fst_zip.
+          2: { rewrite Hlws /logical_region fmap_length; lia. }
+          rewrite /logical_region.
+          intro Hcontra. clear -Hcontra.
+          eapply elem_of_list_fmap_2 in Hcontra.
+          destruct Hcontra as (a & Heq & Hcontra) ; simplify_eq.
+          apply not_elemof_list_remove_elem in Hcontra; auto.
+  Qed.
+
+
+  Lemma mem_map_implies_pure_conds
+    (lmem : LMem) (lregs : LReg) (src : RegName)
+    (a_pc : Addr) (v_pc : Version) (lw_pc : LWord)
+    (p_code : Perm) (b_code e_code a_code : Addr) (v_code : Version)
+    (Ps_code : list D) (has_later : bool) :
+    allow_einit_code_mem lmem lregs src a_pc v_pc lw_pc p_code b_code e_code a_code v_code Ps_code has_later
+    -∗ ⌜lmem !! (a_pc, v_pc) = Some lw_pc⌝.
+  Proof.
+    iIntros "(% & HSweepRes)".
+    rewrite /einit_code_mask_cond.
+    case_decide as Hallows.
+    - pose (Hallows' := Hallows).
+      destruct Hallows' as ((Hreg & Hread) & Hdecide).
+      iDestruct "HSweepRes" as (lws) "(%Hlen & -> & HSweepRest)".
+      by simplify_map_eq.
+    - iDestruct "HSweepRes" as "->".
+      by simplify_map_eq.
+  Qed.
+
+  Lemma allow_einit_code_mem_later
+    (lmem : LMem) (lregs : LReg) (src : RegName)
+    (a_pc : Addr) (v_pc : Version) (lw_pc : LWord)
+    (p_code : Perm) (b_code e_code a_code : Addr) (v_code : Version)
+    (Ps_code : list D) :
+    allow_einit_code_mem lmem lregs src a_pc v_pc lw_pc p_code b_code e_code a_code v_code Ps_code true
+    -∗ ▷ allow_einit_code_mem lmem lregs src a_pc v_pc lw_pc p_code b_code e_code a_code v_code Ps_code false.
+  Proof.
+    iIntros "[% HSweepMem]".
+    rewrite !/allow_einit_code_mem /= /einit_code_mask_cond. iSplit;[auto|].
+    case_decide; last (iNext;iFrame).
+    iApply bi.later_exist_2. iDestruct "HSweepMem" as (lws) "(%&%&HSweepRest)".
+      iExists lws.
+      iDestruct "HSweepRest" as "(?&?&?&?)"; iFrame "%∗"; iNext ; iFrame.
+  Qed.
+
+
+    (* iAssert ( ⌜ *)
+    (*             if ( einit_code_mask_cond (<[PC:=LCap p_pc b_pc e_pc a_pc v_pc]> lregs) src p_src b_src e_src a_src v_src a_pc v_pc ) *)
+    (*             then (∃ dcap, lmem !! (b_src, v_src) = Some dcap) *)
+    (*             else True ⌝ )%I as "%Hdcap". *)
+    (* { *)
+    (*   rewrite /allow_einit_code_mem. *)
+    (*   iDestruct "HEinitCodeMem" as "(_ & HEinitCodeMem)". *)
+    (*   match goal with *)
+    (*   | _ : _ |- context [ einit_code_mask_cond ?regs ?r ?p ?b ?e ?a ?v ?apc ?vpc] => *)
+    (*       set (Hmask := einit_code_mask_cond regs r p b e a v apc vpc) *)
+    (*   end. *)
+    (*   destruct Hmask as [Hmask|] *)
+    (*   ; rewrite /einit_code_mask_cond *)
+    (*   ; [ iEval (rewrite decide_True //) | iEval (rewrite decide_False //)] *)
+    (*   ; last done. *)
+    (*   iDestruct "HEinitCodeMem" as (lws_code) "(%Hlength_lws_code & %Hlmem & _)"; subst. *)
+    (*   iPureIntro. *)
+    (*   destruct Hmask as [Hreg_allow Hcond]. *)
+    (*   destruct Hcond as [-> | Hapc]. *)
+    (*   - rewrite /reg_allows_einit_code in Hreg_allow; simplify_map_eq. *)
+    (*     destruct Hreg_allow as [? ->]; simplify_eq. *)
+    (*     destruct (decide ( b_src = a_src )) as [-> | Hbsrc]. *)
+    (*     + by exists lw_pc; simplify_map_eq. *)
+    (*     + destruct lws_code. *)
+    (*       ++ exfalso. *)
+    (*          cbn in *. *)
+    (*          symmetry in Hlength_lws_code. *)
+    (*          apply length_zero_iff_nil in Hlength_lws_code. *)
+    (*          rewrite /code_addresses in Hlength_lws_code. *)
+    (*          assert (b_src ∈  list_remove_elem a_src (finz.seq_between b_src e_src)) as Hcontra. *)
+    (*          { admit. } *)
+    (*          rewrite Hlength_lws_code in Hcontra. *)
+    (*          set_solver. *)
+    (*       ++ exists l. *)
+    (*          rewrite lookup_insert_ne. *)
+    (*          2:{ intro ; simplify_eq. } *)
+    (*          rewrite /logical_region_map. *)
+    (*          apply elem_of_list_to_map_1. *)
+    (*          admit. *)
+    (*          admit. *)
+    (*   - destruct lws_code. *)
+    (*     ++ exfalso. *)
+    (*        cbn in *. *)
+    (*        symmetry in Hlength_lws_code. *)
+    (*        apply length_zero_iff_nil in Hlength_lws_code. *)
+    (*        rewrite /code_addresses in Hlength_lws_code. *)
+    (*        rewrite list_remove_elem_notin in Hlength_lws_code; auto. *)
+
+    (*        assert (b_src ∈  list_remove_elem a_src (finz.seq_between b_src e_src)) as Hcontra. *)
+    (*          { admit. } *)
+    (*          rewrite Hlength_lws_code in Hcontra. *)
+    (*          set_solver. *)
+    (*       ++ exists l. *)
+    (*          rewrite lookup_insert_ne. *)
+    (*          2:{ intro ; simplify_eq. } *)
+    (*          rewrite /logical_region_map. *)
+    (*          apply elem_of_list_to_map_1. *)
+    (*          admit. *)
+    (*          admit. *)
+
+    (*       by exists lw_pc; simplify_map_eq. *)
+
+
+
+
+    (*   admit. *)
+    (*   + rewrite /einit_code_mask_cond. *)
+    (*   set ( Hmask := (einit_code_mask_cond (<[PC:=LCap p_pc b_pc e_pc a_pc v_pc]> lregs) src p_src b_src e_src a_src v_src a_pc v_pc) ). *)
+    (*   destruct *)
+    (*     (einit_code_mask_cond (<[PC:=LCap p_pc b_pc e_pc a_pc v_pc]> lregs) src p_src b_src e_src *)
+    (*        a_src v_src a_pc v_pc) *)
+    (*       as [Hmask|Hmask]. *)
+
+
+    (* } *)
+
+
+  Lemma einit_case (lregs : leibnizO LReg)
+    (p_pc : Perm) (b_pc e_pc a_pc : Addr) (v_pc : Version)
+    (lw_pc : LWord) (src : RegName) (P : D):
+    ftlr_instr lregs p_pc b_pc e_pc a_pc v_pc lw_pc (EInit src) P.
+  Proof.
+    intros Hp Hsome HcorrectLPC Hbae Hi.
+    iIntros "#IH #Hinv #Hinva #Hreg #(Hread & Hwrite & %HpersP) Hown Ha #HP Hcls HPC Hmap".
+    specialize (HpersP lw_pc).
+    rewrite delete_insert_delete.
+    iDestruct ((big_sepM_delete _ _ PC) with "[HPC Hmap]") as "Hmap /=";
+      [apply lookup_insert|rewrite delete_insert_delete;iFrame|]. simpl.
+
+    (* To read out PC's name later, and needed when calling wp_load *)
+    assert(∀ x : RegName, is_Some (<[PC:=LCap p_pc b_pc e_pc a_pc v_pc]> lregs !! x)) as Hsome'.
+    {
+      intros. destruct (decide (x = PC)) as [Hx|Hx].
+      rewrite Hx lookup_insert; unfold is_Some. by eexists.
+      by rewrite lookup_insert_ne.
+    }
+
+    (* Initializing the names for the values of Hsrc now, to instantiate the existentials in step 1 *)
+    assert (∃ p_src b_src e_src a_src v_src, read_reg_inr (<[PC:=LCap p_pc b_pc e_pc a_pc v_pc]> lregs) src p_src b_src e_src a_src v_src)
+      as (p_src & b_src & e_src & a_src & v_src & HV_Src).
+    {
+      specialize Hsome' with src as Hsrc.
+      destruct Hsrc as [wsrc Hsome_src].
+      unfold read_reg_inr. rewrite Hsome_src.
+      destruct wsrc as [|[ p_src b_src e_src a_src v_src|] | ]; try done.
+      by repeat eexists.
+    }
+
+    (* Step 1: prepare all resources necessary to open the invariants of the argument (the cap given in is_unique), if necessary,
+       and store all the resources obtained from the region in allow_load_res *)
+    iDestruct (create_einit_code_resources with "[$Hreg] [$Hinv]") as (Ps_code) "[%Hlen_Ps HEinitCodeRes]"
+    ; [ eassumption
+      | by apply elem_of_finz_seq_between
+      |].
+
+    (* Open the invariants! *)
+    (* Step 2: derive the concrete map of memory we need, and any spatial predicates holding over it *)
+    iMod (einit_code_resources_implies_mem_map with "HEinitCodeRes Ha") as (lmem) "[HEinitCodeMem HMemCodeRes]".
+    (* rename the big masks to easy names *)
+    set (E0 := ⊤ ∖ ↑logN.@(a_pc, v_pc)).
+    set (E1 := allow_einit_code_mask a_pc v_pc (code_addresses a_pc (finz.seq_between b_src e_src)) v_src).
+
+    (* Step 3:  derive the non-spatial conditions over the memory map*)
+    iDestruct (mem_map_implies_pure_conds with "HEinitCodeMem") as %HReadPC.
+
+    (* Step 4: move the later outside, so that we can remove it after applying wp_isunique *)
+    (* iDestruct (allow_einit_code_mem_later with "HSweepMem") as "HSweepMem"; auto. *)
+
+    iAssert ( ⌜ allows_einit_code (<[PC:=LCap p_pc b_pc e_pc a_pc v_pc]> lregs) src ⌝)%I as "%Hallows_einit_code".
+    { iDestruct "HEinitCodeRes" as "(_&%HeinitCodeRes&_)".
+      iPureIntro. apply HeinitCodeRes.
+    }
+
+    (* iAssert ( ⌜ *)
+    (*             if ( einit_code_mask_cond (<[PC:=LCap p_pc b_pc e_pc a_pc v_pc]> lregs) src p_src b_src e_src a_src v_src a_pc v_pc ) *)
+    (*             then (∃ dcap, lmem !! (b_src, v_src) = Some dcap) *)
+    (*             else True ⌝ )%I as "%Hdcap". *)
+    (* { admit. } *)
+
+
+    Set Nested Proofs Allowed.
+    Fixpoint list_remove_elem_list `{A : Type} `{EqDecision A} (la' la : list A) : list A :=
+      match la' with
+      | [] => la
+      | h::t => list_remove_elem h (list_remove_elem_list t la)
+      end.
+
+    Definition data_addresses (a_pc : Addr) (la_code la_data : list Addr)
+      := (list_remove_elem_list (a_pc::la_code) la_data).
+
+    Definition allow_einit_data_mask
+      (a_pc : Addr) (v_pc : Version)
+      (la_code : list Addr) (v_code : Version)
+      (la_data : list Addr) (v_data : Version)
+      : coPset :=
+      let mask_code := allow_einit_code_mask a_pc v_pc la_code v_code in
+      compute_mask_region mask_code (data_addresses a_pc la_code la_data) v_data.
+
+  Definition read_lmem_inr (lmem : LMem) (a : Addr) (v : Version) p' b' e' a' v' :=
+    match lmem !! (a,v) with
+      | Some (LCap p'' b'' e'' a'' v'') => (LCap p'' b'' e'' a'' v'') = LCap p' b' e' a' v'
+      | Some _ => True
+      | None => False end.
+
+  Definition mem_allows_einit_data
+    (lmem : LMem) (a : Addr) (v : Version)
+    (p' : Perm) (b' e' a' : Addr) (v' : Version):=
+    lmem !! (a,v) = Some (LCap p' b' e' a' v') ∧ p' = RW.
+
+  Definition einit_data_mask_cond
+    (lmem : LMem) (b_code : Addr) (v_code : Version)
+    (p_data : Perm) (b_data e_data a_data : Addr) (v_data : Version)
+    (a_pc : Addr) (v_pc : Version) :=
+    decide (
+        mem_allows_einit_data lmem b_code v_code p_data b_data e_data a_data v_data
+        ∧ a_pc ∉ (finz.seq_between b_data e_data)
+      ).
+
+  Definition interp_list_pred_data
+    (lws : list LWord) (Ps : list D) (has_later : bool) : iProp Σ :=
+    ([∗ list] lw;Pw ∈ lws;Ps, (if has_later then ▷▷ (Pw : D) lw else (Pw : D) lw)).
+
+  Definition interp_list_persistent_data
+    (lws : list LWord) (Ps : list D) : iProp Σ :=
+    ( ⌜ Persistent ([∗ list] lw;Pw ∈ lws;Ps, (Pw : D) lw) ⌝ ).
+
+  Definition interp_list_readcond_data
+    (lws : list LWord) (Ps : list D) (has_later : bool) : iProp Σ :=
+    ( if has_later
+      then [∗ list] Pa ∈ Ps, ▷ read_cond Pa interp
+      else [∗ list] Pa ∈ Ps, (□ ∀ (lw : LWord), (Pa : D) lw -∗ interp lw)
+    )%I.
+
+  Definition interp_list_close_data
+    (la : list Addr) (Ps : list D) (v : Version) (E E' : coPset) : iProp Σ :=
+    ( ▷ (▷ ([∗ list] a_Pa ∈ zip la Ps, (interp_ref_inv a_Pa.1 v a_Pa.2))) ={E', E }=∗ True).
+
+  Definition resources_open_invariant_data
+    (a_pc : Addr) (v_pc : Version)
+    (la_code : list Addr) (v_code : Version)
+    (la_data : list Addr) (v_data : Version) (lws_data : list LWord) (Ps_data : list D)
+    (has_later : bool)
+    : iProp Σ :=
+
+    (* let E0 := ⊤ ∖ ↑logN.@(a_pc, v_pc) in *)
+    let E1 := allow_einit_code_mask a_pc v_pc la_code v_code : coPset in
+    let E2 := allow_einit_data_mask a_pc v_pc la_code v_code la_data v_data : coPset in
+
+    interp_list_pred_data lws_data Ps_data has_later
+    ∗ interp_list_persistent_data lws_data Ps_data
+    ∗ interp_list_readcond_data lws_data Ps_data has_later
+    ∗ interp_list_close_data la_data Ps_data v_data E1 E2.
+
+
+  (* Definition allow_einit_data_resources *)
+  (*   (* (lregs : LReg) *) *)
+  (*   (lmem : LMem) *)
+  (*   (* (src : RegName) *) *)
+  (*   (a_pc : Addr) (v_pc : Version) *)
+  (*   (p_code : Perm) (b_code e_code a_code : Addr) (v_code : Version) (Ps_code : list D) *)
+  (*   (p_data : Perm) (b_data e_data a_data : Addr) (v_data : Version) (Ps_data : list D) *)
+  (*   := *)
+
+  (*   let la_code  := code_addresses a_pc (finz.seq_between b_code e_code) in *)
+  (*   let la_data  := data_addresses a_pc la_code (finz.seq_between b_data e_data) in *)
+  (*   let E0 := ⊤ ∖ ↑logN.@(a_pc, v_pc) in *)
+  (*   let E1 := allow_einit_code_mask a_pc v_pc la_code v_code : coPset in *)
+  (*   let E1' := *)
+  (*     (if einit_code_mask_cond (<[PC:=LCap p_pc b_pc e_pc a_pc v_pc]> lregs) src p_src b_src e_src *)
+  (*           a_src v_src a_pc v_pc then E1 else E0) *)
+  (*   in *)
+  (*   let E2 := allow_einit_data_mask a_pc v_pc la_code v_code la_data v_data : coPset in *)
+
+  (*   ( *)
+  (*     (* ⌜read_reg_inr lregs src p_code b_code e_code a_code v_code⌝ ∗ *) *)
+  (*     ⌜read_lmem_inr lmem b_code v_code p_data b_data e_data a_data v_data⌝ ∗ *)
+  (*     (* ⌜allows_einit_code lregs src⌝ ∗ *) *)
+  (*     ⌜allows_einit_data lmem b_code v_code ⌝ ∗ *)
+  (*    if einit_data_mask_cond lmem b_code v_code p_data b_data e_data a_data v_data a_pc v_pc *)
+  (*    then *)
+  (*     (|={E1, E2}=> (* we open this invariant with all the points-tos from b to e *) *)
+  (*        ∃ (lws_data :list LWord), *)
+  (*        ⌜ length lws_data = length la_data ⌝ *)
+  (*        ∗ ([∗ map] la↦lw ∈ (logical_region_map la_data lws_data v_data), la ↦ₐ lw) (* here you get all the points-tos *) *)
+  (*        ∗ resources_open_invariant_data a_pc v_pc la_code v_code la_data v_data lws_data Ps_data true)%I *)
+  (*    else True)%I. *)
+
+
+    (* Lemma create_einit_data_resources *)
+    (*   (lregs : LReg) (lmem : LMem) (src : RegName) *)
+    (*   (p_pc : Perm) (b_pc e_pc a_pc : Addr) (v_pc : Version) (lw_pc : LWord) *)
+    (*   (p_code : Perm) (b_code e_code a_code : Addr) (v_code : Version) (Ps_code : list D) *)
+    (*   (p_data : Perm) (b_data e_data a_data : Addr) (v_data : Version) : *)
+
+    (*   let la_code  := code_addresses a_pc (finz.seq_between b_code e_code) in *)
+    (*   let la_data  := data_addresses a_pc la_code (finz.seq_between b_data e_data) in *)
+    (*   read_lmem_inr lmem b_code v_code p_data b_data e_data a_data v_data → *)
+
+    (*   (allow_einit_code_resources *)
+    (*      (<[PC:=LCap p_pc b_pc e_pc a_pc v_pc]> lregs) src a_pc v_pc *)
+    (*      p_code b_code e_code a_code v_code Ps_code) -∗ *)
+    (*   (allow_einit_code_mem *)
+    (*     lmem (<[PC:=LCap p_pc b_pc e_pc a_pc v_pc]> lregs) src a_pc v_pc *)
+    (*     lw_pc p_code b_code e_code a_code v_code Ps_code true) -∗ *)
+    (*   ([∗ map] la↦lw ∈ lmem, la ↦ₐ lw) -∗ *)
+
+    (* (∃ (Ps_data : list D), *)
+    (*        ⌜ length la_data = length Ps_data ⌝ *)
+    (*        (* old resources *) *)
+    (*        ∗ (allow_einit_code_resources *)
+    (*             (<[PC:=LCap p_pc b_pc e_pc a_pc v_pc]> lregs) src a_pc v_pc *)
+    (*             p_code b_code e_code a_code v_code Ps_code) *)
+    (*        ∗ (allow_einit_code_mem *)
+    (*             lmem (<[PC:=LCap p_pc b_pc e_pc a_pc v_pc]> lregs) src a_pc v_pc *)
+    (*             lw_pc p_code b_code e_code a_code v_code Ps_code true) *)
+    (*        ∗ ([∗ map] la↦lw ∈ lmem, la ↦ₐ lw) *)
+    (*        (* new resources *) *)
+    (*        ∗ allow_einit_data_resources *)
+    (*            (* (<[PC:=LCap p_pc b_pc e_pc a_pc v_pc]> lregs) *) *)
+    (*            lmem *)
+    (*            (* src *) *)
+    (*            a_pc v_pc *)
+    (*            p_code b_code e_code a_code v_code Ps_code *)
+    (*            p_data b_data e_data a_data v_data Ps_data *)
+    (* ). *)
+    (* Admitted. *)
+
+    (* Initializing the names for the values of Hsrc now, to instantiate the existentials in step 1 *)
+    assert (∃ p_data b_data e_data a_data v_data,
+               read_lmem_inr lmem b_src v_src  p_data b_data e_data a_data v_data)
+      as (p_data & b_data & e_data & a_data & v_data & HV_data).
+    { admit. }
+
+    (* iDestruct (create_einit_data_resources with "[$HEinitCodeRes] [$HEinitCodeMem] [$HMemCodeRes]") *)
+    (*   as (Ps_data) "(%Hlen_Ps_data & _ & HEinitCodeMem & Hmem & HEinitDataRes)"; first eassumption. *)
+
+
+  (* Definition allow_einit_data_mem *)
+  (*   (lmem : LMem) (lregs : LReg) (src : RegName) *)
+  (*   (a_pc : Addr) (v_pc : Version) (lw_pc : LWord) *)
+  (*   (p_code : Perm) (b_code e_code a_code : Addr) (v_code : Version) (Ps_code : list D) (lws_code : list LWord) *)
+  (*   (p_data : Perm) (b_data e_data a_data : Addr) (v_data : Version) (Ps_data : list D) *)
+  (*   (has_later : bool) := *)
+
+  (*   let la_code  := code_addresses a_pc (finz.seq_between b_code e_code) in *)
+  (*   let la_data  := data_addresses a_pc la_code (finz.seq_between b_data e_data) in *)
+
+  (*   ( *)
+  (*     ⌜read_reg_inr lregs src p_code b_code e_code a_code v_code⌝ ∗ *)
+  (*     ⌜read_lmem_inr lmem b_code v_code p_data b_data e_data a_data v_data⌝ ∗ *)
+  (*     if einit_code_mask_cond lregs src p_code b_code e_code a_code v_code a_pc v_pc *)
+  (*     then *)
+  (*       (if einit_data_mask_cond lmem b_code v_code p_data b_data e_data a_data v_data a_pc v_pc *)
+  (*        then *)
+  (*          (∃ (lws_data : list LWord), *)
+  (*              ⌜length lws_data = length la_data⌝ *)
+  (*              ∗ ⌜lmem = <[(a_pc, v_pc):=lw_pc]> *)
+  (*                          (logical_region_map la_code lws_code v_code *)
+  (*                             ∪ logical_region_map la_data lws_data v_data)⌝ *)
+  (*              ∗ resources_open_invariant_data a_pc v_pc la_code v_code la_data v_data lws_data Ps_data has_later)%I *)
+  (*        else ⌜lmem = <[(a_pc, v_pc):=lw_pc]> (logical_region_map la_code lws_code v_code)⌝ *)
+  (*       ) *)
+  (*       ∗ resources_open_invariant_code a_pc v_pc la_code v_code lws_code Ps_code has_later *)
+  (*     else ⌜lmem = <[(a_pc, v_pc):=lw_pc]> ∅⌝)%I. *)
+
+    (* ( *)
+    (*  if einit_code_mask_cond lregs src p_code b_code e_code a_code v_code a_pc v_pc *)
+    (*  then (∃ (lws_code : list LWord), *)
+    (*           ⌜length lws_code = length la_code⌝ *)
+    (*           ∗ ⌜lmem = <[(a_pc, v_pc):=lw_pc]> (logical_region_map la_code lws_code v_code)⌝ *)
+    (*           ∗ resources_open_invariant_code a_pc v_pc la_code v_code lws_code Ps_code has_later)%I *)
+    (*  else ⌜lmem = <[(a_pc, v_pc):=lw_pc]> ∅⌝)%I. *)
+
+  (* Lemma einit_data_resources_implies_mem_map *)
+  (*   (lmem : LMem) (lregs : LReg) (src : RegName) *)
+  (*   (a_pc : Addr) (v_pc : Version) (lw_pc : LWord) *)
+  (*   (p_code : Perm) (b_code e_code a_code : Addr) (v_code : Version) (Ps_code : list D) (lws_code : list LWord) *)
+  (*   (p_data : Perm) (b_data e_data a_data : Addr) (v_data : Version) (Ps_data : list D) : *)
+
+  (*   let la_code  := code_addresses a_pc (finz.seq_between b_code e_code) in *)
+  (*   let la_data  := data_addresses a_pc la_code (finz.seq_between b_data e_data) in *)
+  (*   (* let E0 := ⊤ ∖ ↑logN.@(a_pc, v_pc) in *) *)
+  (*   let E1 := allow_einit_code_mask a_pc v_pc la_code v_code : coPset in *)
+  (*   let E2 := allow_einit_data_mask a_pc v_pc la_code v_code la_data v_data : coPset in *)
+
+  (*   allow_einit_code_resources lregs src a_pc v_pc p_code b_code e_code a_code v_code Ps_code *)
+  (*   allow_einit_data_resources lregs src a_pc v_pc p_code b_code e_code a_code v_code Ps_code *)
+  (*   -∗ (a_pc, v_pc) ↦ₐ lw_pc *)
+  (*   ={ E0, *)
+  (*        if einit_code_mask_cond lregs src p_code b_code e_code a_code v_code a_pc v_pc *)
+  (*        then E1 *)
+  (*        else E0 *)
+  (*     }=∗ *)
+  (*   ∃ lmem : LMem, *)
+  (*     allow_einit_code_mem lmem lregs src a_pc v_pc lw_pc p_code b_code e_code a_code v_code Ps_code true *)
+  (*     ∗ ([∗ map] la↦lw ∈ lmem, la ↦ₐ lw). *)
+
+
+
+
+  (* "HMemCodeRes" : [∗ map] la↦lw ∈ lmem, la ↦ₐ lw *)
+
+
+  (*   iAssert ( ⌜ allows_einit_data lmem  ⌝)%I as "%Hallows_einit_code". *)
+  (*   { iDestruct "HEinitCodeRes" as "(_&%HeinitCodeRes&_)". *)
+  (*     iPureIntro. apply HeinitCodeRes. *)
+  (*   } *)
+
+  (*   iApply (wp_einit with "[$Hmap $HMemCodeRes]") *)
+  (*   ; eauto *)
+  (*   ; [ by simplify_map_eq *)
+  (*     | rewrite /subseteq /map_subseteq /set_subseteq_instance *)
+  (*       ; intros rr _; apply elem_of_dom *)
+  (*       ; rewrite lookup_insert_is_Some'; *)
+  (*       eauto *)
+  (*     | | | ]. *)
+
   Admitted.
+
+
+
+
+
+
+  (* (** Predicate that defines when the contents of a register can be swept; *)
+  (*     i.e. when the register contains a capability with at least R permissions... *) *)
+  (* Definition reg_allows_einit *)
+  (*   (lregs : LReg) (lmem : LMem) (r : RegName) *)
+  (*   (b e a : Addr) (v : Version) *)
+  (*   (b' e' a' : Addr) (v' : Version):= *)
+  (*   lregs !! r = Some (LCap RX b e a v) *)
+  (*   ∧ lmem !! (a,v) = Some (LCap RW b' e' a' v'). *)
+
+  (* (* TODO move stdpp_extra *) *)
+  (* Fixpoint list_remove_elem_list `{A : Type} `{EqDecision A} (la' la : list A) : list A := *)
+  (*   match la' with *)
+  (*   | [] => la *)
+  (*   | h::t => list_remove_elem h (list_remove_elem_list t la) *)
+  (*   end. *)
+
+  (* Definition code_addresses (a_pc : Addr) (code_la : list Addr) *)
+  (*   := (list_remove_elem a_pc code_la). *)
+
+  (* Definition allow_einit_mask_code *)
+  (*   (a_pc : Addr) (v_pc : Version) *)
+  (*   (code_la : list Addr) (code_v : Version) *)
+  (*   : coPset := *)
+  (*   let pc_mask := (⊤ ∖ ↑logN.@(a_pc, v_pc)) in *)
+  (*   compute_mask_region pc_mask (code_addresses a_pc code_la) code_v. *)
+
+  (* Definition data_addresses (a_pc : Addr) (code_la data_la : list Addr) *)
+  (*   := (list_remove_elem_list (a_pc::code_la) data_la). *)
+
+  (* Definition allow_einit_mask_data *)
+  (*   (a_pc : Addr) (v_pc : Version) *)
+  (*   (code_la : list Addr) (code_v : Version) *)
+  (*   (data_la : list Addr) (data_v : Version) *)
+  (*   : coPset := *)
+  (*   let code_mask := allow_einit_mask_code a_pc v_pc code_la code_v in *)
+  (*   compute_mask_region code_mask (data_addresses a_pc code_la data_la) data_v. *)
+
+  (* (* Lemma allow_einit_mask_remove_nodup *) *)
+  (* (*   (a_pc : Addr) (v_pc : Version) (code_la data_la : list Addr) (v : Version) : *) *)
+  (* (*   NoDup code_la -> *) *)
+  (* (*   NoDup data_la -> *) *)
+  (* (*   allow_sweep_mask a_pc v_pc (list_remove_elem a_pc la) v = *) *)
+  (* (*   allow_sweep_mask a_pc v_pc la v. *) *)
+  (* (* Proof. *) *)
+  (* (*   intros HNoDup. *) *)
+  (* (*   by rewrite /allow_sweep_mask list_remove_elem_idem. *) *)
+  (* (* Qed. *) *)
+
+  (* (* this will help us close the invariant again... *) *)
+  (* (* it states which properties are enforced on all the lws *) *)
+
+
+  (* Definition region_open_resources *)
+  (*   (a_pc : Addr) (v_pc : Version) *)
+  (*   (code_la : list Addr) (code_v : Version) *)
+  (*   (code_lws : list LWord) (code_Ps : list D) *)
+  (*   (data_la : list Addr) (data_v : Version) *)
+  (*   (data_lws : list LWord) (data_Ps : list D) *)
+  (*   (has_later : bool) *)
+  (*   : iProp Σ := *)
+
+  (*   let E := ⊤ ∖ ↑logN.@(a_pc, v_pc) in *)
+  (*   let E1 := allow_einit_mask_code a_pc v_pc code_la code_v in *)
+  (*   let E2 := allow_einit_mask_data a_pc v_pc code_la code_v data_la data_v in *)
+
+  (*   ([∗ list] lw;Pw ∈ code_lws;code_Ps, (if has_later then ▷ (Pw : D) lw else (Pw : D) lw)) *)
+  (*   ∗ ([∗ list] lw;Pw ∈ data_lws;data_Ps, (if has_later then ▷▷ (Pw : D) lw else (Pw : D) lw)) *)
+
+  (*   ∗ ( ⌜ Persistent ([∗ list] lw;Pw ∈ code_lws;code_Ps, (Pw : D) lw) ⌝ ) (* All properties P are persistent *) *)
+  (*   ∗ ( ⌜ Persistent ([∗ list] lw;Pw ∈ data_lws;data_Ps, (Pw : D) lw) ⌝ ) (* All properties P are persistent *) *)
+
+  (*   ∗ ( if has_later *)
+  (*       then ([∗ list] Pa ∈ code_Ps, read_cond Pa interp) *)
+  (*            ∗ ([∗ list] Pa ∈ data_Ps, ▷ read_cond Pa interp) *)
+  (*              (* the read cond holds *) *)
+  (*       else ([∗ list] Pa ∈ code_Ps, (□ ∀ (lw : LWord), (Pa : D) lw -∗ interp lw)) *)
+  (*              ∗ ([∗ list] Pa ∈ data_Ps, (□ ∀ (lw : LWord), (Pa : D) lw -∗ interp lw)) *)
+  (*     )%I *)
+
+  (*   ∗ (▷▷ ([∗ list] a_Pa ∈ zip data_la code_Ps, (interp_ref_inv a_Pa.1 data_v a_Pa.2)) ={E2, E1 }=∗ True) *)
+  (*   ∗ (▷ ([∗ list] a_Pa ∈ zip code_la data_Ps, (interp_ref_inv a_Pa.1 code_v a_Pa.2)) ={E1, E }=∗ True). *)
+
+  (* Definition einit_mask_cond *)
+  (*   (lregs : LReg) (lmem : LMem) *)
+  (*   (src : RegName) (b_code e_code a_code : Addr) (v_code : Version) *)
+  (*   (b_data e_data a_data : Addr) (v_data : Version) *)
+  (*   (a_pc : Addr) (v_pc : Version) := *)
+  (*   decide (reg_allows_einit lregs lmem src b_code e_code a_code v_code b_data e_data a_data v_data *)
+  (*           /\ (src = PC \/ a_pc ∉ (finz.seq_between b_code e_code)) *)
+  (*           /\ a_pc ∉ (finz.seq_between b_data e_data) *)
+  (*     ). *)
+
+  (* (* Description of what the resources are supposed to look like after opening the region *) *)
+  (* (*    if we need to, but before closing the region up again*) *)
+
+  (* Definition allow_einit_res *)
+  (*   (lregs : LReg) (lmem : LMem) *)
+  (*   (src : RegName) *)
+  (*   (a_pc : Addr) (v_pc : Version) *)
+  (*   (b_code e_code a_code : Addr) (v_code : Version) (code_Ps : list D) *)
+  (*   (b_data e_data a_data : Addr) (v_data : Version) (data_Ps : list D) *)
+  (*   := *)
+
+  (*   let code_la  := code_addresses a_pc (finz.seq_between b_code e_code) in *)
+  (*   let data_la  := data_addresses a_pc code_la (finz.seq_between b_data e_data) in *)
+  (*   let E   := ⊤ ∖ ↑logN.@(a_pc, v_pc) in *)
+  (*   let E1 := allow_einit_mask_code a_pc v_pc code_la v_code in *)
+  (*   let E2 := allow_einit_mask_data a_pc v_pc code_la v_code data_la v_data in *)
+
+  (*   (⌜read_reg_inr lregs src RX b_code e_code a_code v_code⌝ ∗ *)
+  (*    ⌜allows_einit lregs lmem src⌝ ∗ *)
+  (*    if einit_mask_cond lregs lmem *)
+  (*         src b_code e_code a_code v_code *)
+  (*         b_data e_data a_data v_data *)
+  (*         a_pc v_pc *)
+  (*    then *)
+  (*     (|={E, E2}=> (* we open this invariant with all the points-tos from b to e *) *)
+  (*        ∃ (code_lws : list LWord) (data_lws : list LWord), *)
+  (*        ⌜ length code_lws = length code_la ⌝ *)
+  (*        ∗ ⌜ length data_lws = length data_la ⌝ *)
+  (*        ∗ ([∗ map] la↦lw ∈ (logical_region_map code_la code_lws v_code), la ↦ₐ lw) (* here you get all the points-tos *) *)
+  (*        ∗ ([∗ map] la↦lw ∈ (logical_region_map data_la data_lws v_data), la ↦ₐ lw) *)
+  (*        ∗ region_open_resources a_pc v_pc *)
+  (*            code_la v_code code_lws code_Ps *)
+  (*            data_la v_data data_lws data_Ps *)
+  (*            true)%I *)
+  (*    else True)%I. *)
+
+  (* (* this does not yet open the invariant *) *)
+  (* Lemma create_einit_res *)
+  (*   (lregs : LReg) (lmem : LMem) *)
+  (*   (src : RegName) *)
+  (*   (p_pc : Perm) (b_pc e_pc a_pc : Addr) (v_pc : Version) *)
+  (*   (b_code e_code a_code : Addr) (v_code : Version) *)
+  (*   (b_data e_data a_data : Addr) (v_data : Version) : *)
+
+  (*   let code_la  := code_addresses a_pc (finz.seq_between b_code e_code) in *)
+  (*   let data_la  := data_addresses a_pc code_la (finz.seq_between b_data e_data) in *)
+
+  (*   read_reg_inr (<[PC:=LCap p_pc b_pc e_pc a_pc v_pc]> lregs) src RX b_code e_code a_code v_code *)
+  (*   -> a_pc ∈ finz.seq_between b_pc e_pc *)
+  (*   → (∀ (r : RegName) lw, ⌜r ≠ PC⌝ → ⌜lregs !! r = Some lw⌝ → (fixpoint interp1) lw) *)
+  (*   -∗ interp (LCap p_pc b_pc e_pc a_pc v_pc) *)
+  (*   -∗ (∃ (code_Ps : list D) (data_Ps  : list D), *)
+  (*          ⌜ length code_la = length code_Ps ⌝ *)
+  (*          ∗ ⌜length data_la = length data_Ps ⌝ *)
+  (*          ∗ allow_einit_res *)
+  (*              (<[PC:=LCap p_pc b_pc e_pc a_pc v_pc]> lregs) lmem src *)
+  (*              a_pc v_pc *)
+  (*              b_code e_code a_code v_code code_Ps *)
+  (*              b_data e_data a_data v_data data_Ps *)
+  (*      ). *)
+  (* Proof. *)
+  (* Admitted. *)
+
+  (* Definition allow_einit_mem *)
+  (*   (lmem : LMem) (lregs : LReg) (src : RegName) *)
+  (*   (a_pc : Addr) (v_pc : Version) (lw_pc : LWord) *)
+
+  (*   (b_code e_code a_code : Addr) (v_code : Version) (code_Ps : list D) *)
+  (*   (b_data e_data a_data : Addr) (v_data : Version) (data_Ps : list D) *)
+
+  (*   (has_later : bool) := *)
+
+  (*   let code_la  := code_addresses a_pc (finz.seq_between b_code e_code) in *)
+  (*   let data_la  := data_addresses a_pc code_la (finz.seq_between b_data e_data) in *)
+
+  (*   (⌜read_reg_inr lregs src RX b_code e_code a_code v_code⌝ ∗ *)
+  (*    if einit_mask_cond lregs lmem *)
+  (*         src b_code e_code a_code v_code *)
+  (*         b_data e_data a_data v_data *)
+  (*         a_pc v_pc *)
+  (*    then (∃ (code_lws : list LWord) (data_lws : list LWord), *)
+  (*          ⌜ length code_la = length code_lws ⌝ *)
+  (*          ∗ ⌜length data_la = length data_lws ⌝ *)
+  (*          ∗ ⌜lmem = <[(a_pc, v_pc):=lw_pc]> *)
+  (*                      (logical_region_map code_la code_lws v_code *)
+  (*                         ∪ logical_region_map data_la data_lws v_data)⌝ *)
+  (*             ∗ region_open_resources a_pc v_pc *)
+  (*                 code_la v_code code_lws code_Ps *)
+  (*                 data_la v_data data_lws data_Ps *)
+  (*                 has_later) *)
+  (*    else ⌜lmem = <[(a_pc, v_pc):=lw_pc]> ∅⌝)%I. *)
+
+  (* (* Create the lmem with the points-tos we need for the is_unique case *) *)
+  (* Lemma einit_res_implies_mem_map *)
+  (*   (lregs : LReg) (lmem : LMem) (src : RegName) *)
+  (*   (a_pc : Addr) (v_pc : Version) (lw_pc : LWord) *)
+
+  (*   (b_code e_code a_code : Addr) (v_code : Version) (code_Ps : list D) *)
+  (*   (b_data e_data a_data : Addr) (v_data : Version) (data_Ps : list D) : *)
+
+  (*   let code_la  := code_addresses a_pc (finz.seq_between b_code e_code) in *)
+  (*   let data_la  := data_addresses a_pc code_la (finz.seq_between b_data e_data) in *)
+
+  (*   let E   := ⊤ ∖ ↑logN.@(a_pc, v_pc) in *)
+  (*   let E1 := allow_einit_mask_code a_pc v_pc code_la v_code in *)
+  (*   let E2 := allow_einit_mask_data a_pc v_pc code_la v_code data_la v_data in *)
+
+  (*   allow_einit_res lregs src a_pc v_pc lw_pc *)
+  (*     b_code e_code a_code v_code code_Ps *)
+  (*     b_data e_data a_data v_data data_Ps *)
+  (*   -∗ (a_pc, v_pc) ↦ₐ lw_pc *)
+  (*   ={ E, *)
+  (*        if einit_mask_cond lregs *)
+  (*         src b_code e_code a_code v_code *)
+  (*         b_data e_data a_data v_data *)
+  (*         a_pc v_pc *)
+  (*        then E2 *)
+  (*        else E *)
+  (*     }=∗ *)
+  (*   ∃ lmem : LMem, *)
+  (*     allow_einit_mem lmem lregs src a_pc v_pc lw_pc *)
+  (*                     b_code e_code a_code v_code code_Ps *)
+  (*                     b_data e_data a_data v_data data_Ps *)
+  (*                     true *)
+  (*     ∗ ([∗ map] la↦lw ∈ lmem, la ↦ₐ lw). *)
+  (* Proof. *)
+  (*   intros *. *)
+  (*   iIntros "HSweepRes Ha_pc". *)
+  (*   iDestruct "HSweepRes" as "(%Hread & [ %Hreserved HSweepRes ] )". *)
+  (*   subst E'. *)
+  (*   rewrite /sweep_mask_cond. *)
+  (*   case_decide as Hallows; cycle 1. *)
+  (*     - iExists _. *)
+  (*       iSplitR "Ha_pc". *)
+  (*       + iFrame "%". *)
+  (*         rewrite /sweep_mask_cond; case_decide; first by exfalso. auto. *)
+  (*       + iModIntro; iNext. by iApply memMap_resource_1. *)
+  (*     - iMod "HSweepRes" as (lws) "(%Hlws & Hmem & HSweepRest)". *)
+  (*       iExists _. *)
+  (*       iSplitL "HSweepRest". *)
+  (*       * iFrame "%". *)
+  (*         rewrite decide_True; auto. *)
+  (*       * iModIntro;iNext. *)
+  (*         destruct Hallows as ((Hrinr & Hra) & Hne). *)
+  (*         iDestruct (big_sepM_insert with "[$Hmem $Ha_pc]") as "Hmem" ; cycle 1 ; auto. *)
+  (*         rewrite /logical_region_map. *)
+  (*         apply not_elem_of_list_to_map_1. *)
+  (*         rewrite fst_zip. *)
+  (*         2: { rewrite Hlws /logical_region fmap_length; lia. } *)
+  (*         rewrite /logical_region. *)
+  (*         intro Hcontra. clear -Hcontra. *)
+  (*         eapply elem_of_list_fmap_2 in Hcontra. *)
+  (*         destruct Hcontra as (a & Heq & Hcontra) ; simplify_eq. *)
+  (*         apply not_elemof_list_remove_elem in Hcontra; auto. *)
+  (* Qed. *)
+
+
 
 End fundamental.
